coq-osiris/theories/proofmode/pure_eval.v
@@ -10,8 +10,8 @@ From osiris.proofmode Require Import simp_tactics.
 (* TODO can we give a similar lemma at arity [n]? *)
 
 Lemma pure_eval_pair `{Encode A1, Encode A2} η e1 e2 (ψ : A1 * A2 → Prop) :
-  pure_enc (eval η e1) (λ a1 : A1, pure_enc (eval η e2) (λ a2 : A2, ψ (a1, a2))) →
-  pure_enc (eval η (EPair e1 e2)) ψ.
+  pure (eval η e1) ##(λ a1 : A1, pure (eval η e2) ##(λ a2 : A2, ψ (a1, a2)) ⊥) ⊥ →
+  pure (eval η (EPair e1 e2)) ##ψ ⊥.
 Proof.
   intros. simpl_eval.
   eapply purev_Par_left_conseq; eauto. intros ? (? & -> & ?).
@@ -21,11 +21,11 @@ Proof.
 Qed.
 
 Lemma pure_eval_triple `{Encode A1, Encode A2, Encode A3} η e1 e2 e3 (ψ : A1 * A2 * A3 -> Prop) :
-  pure_enc (eval η e1) (λ a1 : A1,
-        pure_enc (eval η e2) (λ a2 : A2,
-              pure_enc (eval η e3) (λ a3 : A3,
-                    ψ (a1, a2, a3)))) ->
-  pure_enc (eval η (ETuple [e1; e2; e3])) ψ.
+  pure (eval η e1) ##(λ a1 : A1,
+        pure (eval η e2) ##(λ a2 : A2,
+              pure (eval η e3) ##(λ a3 : A3,
+                    ψ (a1, a2, a3)) ⊥) ⊥) ⊥ ->
+  pure (eval η (ETuple [e1; e2; e3])) ##ψ ⊥.
 Proof.
   intros. simpl_eval.
   eapply purev_Par_left_conseq; eauto. intros ? (? & -> & ?).
@@ -37,12 +37,12 @@ Qed.
 
 Lemma pure_eval_quadruple `{Encode A1, Encode A2, Encode A3, Encode A4} (η : env) (e1 e2 e3 e4 : expr)
   (ψ : A1 * A2 * A3 * A4 → Prop) :
-  pure_enc (eval η e1) (λ a1 : A1,
-        pure_enc (eval η e2) (λ a2 : A2,
-              pure_enc (eval η e3) (λ a3 : A3,
-                    pure_enc (eval η e4) (λ a4 : A4,
-                          ψ (a1, a2, a3, a4))))) ->
-  pure_enc (eval η (ETuple [e1; e2; e3; e4])) ψ.
+  pure (eval η e1) ##(λ a1 : A1,
+        pure (eval η e2) ##(λ a2 : A2,
+              pure (eval η e3) ##(λ a3 : A3,
+                    pure (eval η e4) ##(λ a4 : A4,
+                          ψ (a1, a2, a3, a4)) ⊥) ⊥) ⊥) ⊥ ->
+  pure (eval η (ETuple [e1; e2; e3; e4])) ##ψ ⊥.
 Proof.
   intros. simpl_eval.
   eapply purev_Par_left_conseq; eauto. intros ? (? & -> & ?).
@@ -54,35 +54,35 @@ Proof.
 Qed.
 
 Lemma pure_eval_pair_val η e1 e2 (ψ : val → Prop) :
-  pure_enc (eval η e1) (λ a1 : val, pure_enc (eval η e2) (λ a2 : val, ψ (VPair a1 a2))) →
-  pure_enc (eval η (EPair e1 e2)) ψ.
+  pure (eval η e1) ##(λ a1 : val, pure (eval η e2) ##(λ a2 : val, ψ (VPair a1 a2)) ⊥) ⊥ →
+  pure (eval η (EPair e1 e2)) ##ψ ⊥.
 Proof.
   intros. simpl_eval.
   eapply purev_Par_left_conseq; eauto. intros ? (? & -> & ?).
   eapply purev_Par_left_conseq; eauto. intros ? (? & -> & ?).
   repeat apply pure_ret.
-  eauto.
+  eauto with encode.
 Qed.
 
 Lemma pure_eval_pair_conseq `{Encode A1, Encode A2} η e1 e2
   (φ1 : A1 → Prop) (φ2 : A2 → Prop) (ψ : A1 * A2 → Prop)
 :
-  pure_enc (eval η e1) φ1 →
-  pure_enc (eval η e2) φ2 →
+  pure (eval η e1) ##φ1 ⊥ →
+  pure (eval η e2) ##φ2 ⊥ →
   (∀ a1 a2, φ1 a1 → φ2 a2 → ψ (a1, a2)) →
-  pure_enc (eval η (EPair e1 e2)) ψ.
+  pure (eval η (EPair e1 e2)) ##ψ ⊥.
 Proof.
   intros. simpl_eval.
   eapply purev_Par_left_conseq; eauto. intros ? (? & -> & ?).
   eapply purev_Par_left_conseq; eauto. intros ? (? & -> & ?).
-  repeat apply pure_ret. eauto with encode.
+  repeat apply pure_ret. eauto 10 with encode.
 Qed.
 
 (* TODO: comment *)
 
 Lemma pure_eval_int η i (ψ : Z -> Prop) :
   ψ i ->
-  pure_enc (eval η (EInt i)) ψ.
+  pure (eval η (EInt i)) ##ψ ⊥.
 Proof.
   intros.
   eapply pure_simp. simp.
@@ -92,9 +92,9 @@ Qed.
 (* Function applications. *)
 
 Lemma pure_eval_anonfun `{Encode A, Encode A1} η v e (φ : A1 -> Prop) (ψ : val -> Prop) :
-  (∀ (x : A), pure_enc (eval ((v, #x) :: η) e) φ) ->
-  (∀ (vf : val), (∀ (x : A), pure_enc (call vf #x) φ) -> ψ vf) ->
-  pure_enc (eval η (EAnonFun (AnonFun v e))) ψ.
+  (∀ (x : A), pure (eval ((v, #x) :: η) e) ##φ ⊥) ->
+  (∀ (vf : val), (∀ (x : A), pure (call vf #x) ##φ ⊥) -> ψ vf) ->
+  pure (eval η (EAnonFun (AnonFun v e))) ##ψ ⊥.
 Proof.
   intros Hcall Hcov. specialize (Hcov (VClo η (AnonFun v e))).
   eapply pure_simp; [ simp | eauto ].
@@ -106,7 +106,7 @@ Qed.
 Lemma pure_eval_anonfun' `{Encode A, Encode A1} η a φ (ψ : val -> Prop) :
   (∀ (x : A), φ (VClo η a) #x) ->
   (∀ (vf : val), (∀ (x : A), φ vf #x) -> ψ vf) ->
-  pure_enc (eval η (EAnonFun a)) ψ.
+  pure (eval η (EAnonFun a)) ##ψ ⊥.
 Proof.
   intros Hcall Hcov. specialize (Hcov (VClo η a)).
   eapply pure_simp; [ simp | eauto ].
@@ -116,11 +116,11 @@ Qed.
 
 Lemma pure_eval_anonfunction `{Encode A, Encode A1} η bs (φ : A1 -> Prop) (ψ : val -> Prop) :
   (∀ (x : A),
-      pure_enc
+      pure
         (deep_eval_match (("__osiris_anonymous_arg", #x) :: η) bs (O2Ret #x))
-        φ) ->
-  (∀ (vf : val), (∀ (x : A), pure_enc (call vf #x) φ) -> ψ vf) ->
-  pure_enc (eval η (EAnonFun (AnonFunction bs))) ψ.
+        ##φ ⊥) ->
+  (∀ (vf : val), (∀ (x : A), pure (call vf #x) ##φ ⊥) -> ψ vf) ->
+  pure (eval η (EAnonFun (AnonFunction bs))) ##ψ ⊥.
 Proof.
   intros Hcall Hcov.
   eapply pure_simp; [ simp | eauto ].
@@ -131,12 +131,12 @@ Proof.
 Qed.
 
 Lemma pure_eval_app `{Encode A1, Encode A} η e1 e2 (ψ : A → Prop) :
-  pure_enc (eval η e1)
-    (λ f : val,
-        pure_enc (eval η e2)
-          (λ arg : A1,
-              pure_enc (call f #arg) ψ)) →
-  pure_enc (eval η (EApp e1 e2)) ψ.
+  pure (eval η e1)
+    ##(λ f : val,
+        pure (eval η e2)
+          ##(λ arg : A1,
+              pure (call f #arg) ##ψ ⊥) ⊥) ⊥ →
+  pure (eval η (EApp e1 e2)) ##ψ ⊥.
 Proof.
   intros He1. simpl_eval.
   apply pure_Par_vals_left.
@@ -148,10 +148,10 @@ Qed.
 Lemma pure_eval_app_conseq `{Encode A, Encode B} η e1 e2
   (φ1 : val → Prop) (φ2 : A → Prop) (ψ : B → Prop)
 :
-  pure_enc (eval η e1) φ1 →
-  pure_enc (eval η e2) φ2 →
-  (∀ v1 v2, φ1 v1 → φ2 v2 → pure_enc (call v1 #v2) ψ) →
-  pure_enc (eval η (EApp e1 e2)) ψ.
+  pure (eval η e1) ##φ1 ⊥ →
+  pure (eval η e2) ##φ2 ⊥ →
+  (∀ v1 v2, φ1 v1 → φ2 v2 → pure (call v1 #v2) ##ψ ⊥) →
+  pure (eval η (EApp e1 e2)) ##ψ ⊥.
 Proof.
   intros He1 He2 Hp. simpl_eval.
   apply pure_Par_vals_left.
@@ -160,18 +160,19 @@ Proof.
   apply Hp; eauto with encode.
 Qed.
 
+(* TODO redundant with pure_hoare.v's pure_call2? *)
 Definition pure_call2 `{Encode X} vf arg1 arg2 (φ : X -> Prop) :=
-  pure_enc (call vf arg1)
-    (λ c, pure_enc (call c arg2) φ).
+  pure (call vf arg1)
+    ##(λ c, pure (call c arg2) ##φ ⊥) ⊥.
 
 Lemma pure_eval_app2 `{Encode A, Encode B, Encode C} η e1 e2 e3 vf
   (arg1 : A) (arg2 : B) (ψ : C → Prop)
   :
-  pure_enc (eval η e1) (λ vf', vf' = vf) ->
-  pure_enc (eval η e2) (λ arg1', arg1' = arg1) ->
-  pure_enc (eval η e3) (λ arg2', arg2' = arg2) ->
+  pure (eval η e1) ##(λ vf', vf' = vf) ⊥ ->
+  pure (eval η e2) ##(λ arg1', arg1' = arg1) ⊥ ->
+  pure (eval η e3) ##(λ arg2', arg2' = arg2) ⊥ ->
   pure_call2 vf #arg1 #arg2 ψ ->
-  pure_enc (eval η (EApp (EApp e1 e2) e3)) ψ.
+  pure (eval η (EApp (EApp e1 e2) e3)) ##ψ ⊥.
 Proof.
   intros He1 He2 He3 Hcall.
   eapply pure_simp; [ simp | eauto ].
@@ -181,18 +182,18 @@ Proof.
   apply (pure_mono_ret _ He2). intros ? (? & -> & ->).
   apply (pure_mono_ret _ Hcall). intros ? (c & -> & Hc).
   apply (pure_mono_ret _ He3). intros ? (? & -> & ->).
-  auto.
+  auto with encode.
 Qed.
 
 Lemma pure_eval_app2_conseq `{Encode A, Encode B, Encode C} η e1 e2 e3 vf
   (arg1 : A) (arg2 : B) (φ ψ : C → Prop)
   :
-  pure_enc (eval η e1) (λ vf', vf' = vf) ->
-  pure_enc (eval η e2) (λ arg1', arg1' = arg1) ->
-  pure_enc (eval η e3) (λ arg2', arg2' = arg2) ->
+  pure (eval η e1) ##(λ vf', vf' = vf) ⊥ ->
+  pure (eval η e2) ##(λ arg1', arg1' = arg1) ⊥ ->
+  pure (eval η e3) ##(λ arg2', arg2' = arg2) ⊥ ->
   pure_call2 vf #arg1 #arg2 φ ->
   (∀ a, φ a → ψ a) →
-  pure_enc (eval η (EApp (EApp e1 e2) e3)) ψ.
+  pure (eval η (EApp (EApp e1 e2) e3)) ##ψ ⊥.
 Proof.
   intros.
   eapply pure_eval_app2; eauto.
@@ -204,8 +205,8 @@ Qed.
 (* Helper lemmas for arithmetic operations. *)
 
 Lemma pure_as_int m (φ : Z → Prop) :
-  pure_enc m φ →
-  pure (as_int m) (λ i, ∃ z, i = repr z ∧ φ z) (λ _, False).
+  pure m ##φ ⊥ →
+  pure (as_int m) (λ i, ∃ z, i = repr z ∧ φ z) ⊥.
 Proof.
   intros Hm. apply pure_bind.
   apply (pure_mono_ret _ Hm). intros ? (z & -> & Hz).
@@ -213,14 +214,14 @@ Proof.
 Qed.
 
 Lemma pure_enc_par_as_int m1 m2 (φ1 φ2 φ : Z → Prop) k :
-  pure_enc m1 φ1 →
-  pure_enc m2 φ2 →
-  (∀ z1 z2 : Z, φ1 z1 → φ2 z2 → pure_enc (k (repr z1, repr z2)) φ) →
-  pure_enc (Par (as_int m1) (as_int m2) (pfbind inject2 k)) φ.
+  pure m1 ##φ1 ⊥ →
+  pure m2 ##φ2 ⊥ →
+  (∀ z1 z2 : Z, φ1 z1 → φ2 z2 → pure (k (repr z1, repr z2)) ##φ ⊥) →
+  pure (Par (as_int m1) (as_int m2) (pfbind inject2 k)) ##φ ⊥.
 Proof.
   intros Hm1 Hm2 Hk.
   unfold as_int.
-  eapply pure_Par_conseq. 1,2: eapply pure_as_int; eauto. 2: tauto.
+  eapply pure_Par_conseq. 1,2: eapply pure_as_int; eauto. 2: firstorder.
   intros ? ? (z1 & -> & Hz1) (z2 & -> & Hz2).
   eapply pure_simp; [ simp | ].
   by apply Hk.
@@ -229,43 +230,43 @@ Qed.
 (* Primitive arithmetic operations. *)
 
 Lemma pure_eval_add η e1 e2 (φ1 φ2 φ : Z → Prop) :
-  pure_enc (eval η e1) φ1 →
-  pure_enc (eval η e2) φ2 →
+  pure (eval η e1) ##φ1 ⊥ →
+  pure (eval η e2) ##φ2 ⊥ →
   (∀ z1 z2, φ1 z1 → φ2 z2 → φ (z1 + z2)) →
-  pure_enc (eval η (EIntAdd e1 e2)) φ.
+  pure (eval η (EIntAdd e1 e2)) ##φ ⊥.
 Proof.
   intros. simpl_eval. eapply pure_enc_par_as_int; eauto. intros.
   eapply pure_enc_ret; eauto with encode.
 Qed.
 
 Lemma pure_eval_sub η e1 e2 (φ1 φ2 φ : Z → Prop) :
-  pure_enc (eval η e1) φ1 →
-  pure_enc (eval η e2) φ2 →
+  pure (eval η e1) ##φ1 ⊥ →
+  pure (eval η e2) ##φ2 ⊥ →
   (∀ z1 z2, φ1 z1 → φ2 z2 → φ (z1 - z2)) →
-  pure_enc (eval η (EIntSub e1 e2)) φ.
+  pure (eval η (EIntSub e1 e2)) ##φ ⊥.
 Proof.
   intros. simpl_eval. eapply pure_enc_par_as_int; eauto. intros.
   eapply pure_enc_ret; eauto with encode.
 Qed.
 
 Lemma pure_eval_mul η e1 e2 (φ1 φ2 φ : Z → Prop) :
-  pure_enc (eval η e1) φ1 →
-  pure_enc (eval η e2) φ2 →
+  pure (eval η e1) ##φ1 ⊥ →
+  pure (eval η e2) ##φ2 ⊥ →
   (∀ z1 z2, φ1 z1 → φ2 z2 → φ (z1 * z2)) →
-  pure_enc (eval η (EIntMul e1 e2)) φ.
+  pure (eval η (EIntMul e1 e2)) ##φ ⊥.
 Proof.
   intros. simpl_eval. eapply pure_enc_par_as_int; eauto. intros.
   eapply pure_enc_ret; eauto with encode.
 Qed.
 
 Lemma pure_eval_div η e1 e2 (φ1 φ2 φ : Z → Prop) :
-  pure_enc (eval η e1) φ1 →
-  pure_enc (eval η e2) φ2 →
+  pure (eval η e1) ##φ1 ⊥ →
+  pure (eval η e2) ##φ2 ⊥ →
   (∀ z1, φ1 z1 → representable z1) →
   (∀ z2, φ2 z2 → representable z2) →
   (∀ z2, φ2 z2 → z2 ≠ 0) →
   (∀ z1 z2, φ1 z1 → φ2 z2 → φ (z1 ÷ z2)) →
-  pure_enc (eval η (EIntDiv e1 e2)) φ.
+  pure (eval η (EIntDiv e1 e2)) ##φ ⊥.
 Proof.
   intros. simpl_eval. eapply pure_enc_par_as_int; eauto. intros.
   eapply pure_bind, pure_mono_ret.
@@ -278,9 +279,9 @@ Qed.
 (* Primitive logical operations on machine integers. *)
 
 Lemma pure_eval_lnot η e1 (φ1 φ : Z → Prop) :
-  pure_enc (eval η e1) φ1 →
+  pure (eval η e1) ##φ1 ⊥ →
   (∀ z1, φ1 z1 → φ (Z.lnot z1)) →
-  pure_enc (eval η (EIntLnot e1)) φ.
+  pure (eval η (EIntLnot e1)) ##φ ⊥.
 Proof.
   intros He1%pure_as_int Hp. simpl_eval.
   eapply pure_bind_conseq; eauto. intros ? (z & -> & Hz).
@@ -288,42 +289,42 @@ Proof.
 Qed.
 
 Lemma pure_eval_land η e1 e2 (φ1 φ2 φ : Z → Prop) :
-  pure_enc (eval η e1) φ1 →
-  pure_enc (eval η e2) φ2 →
+  pure (eval η e1) ##φ1 ⊥ →
+  pure (eval η e2) ##φ2 ⊥ →
   (∀ z1 z2, φ1 z1 → φ2 z2 → φ (Z.land z1 z2)) →
-  pure_enc (eval η (EIntLand e1 e2)) φ.
+  pure (eval η (EIntLand e1 e2)) ##φ ⊥.
 Proof.
   intros. simpl_eval. eapply pure_enc_par_as_int; eauto. intros.
   eapply pure_enc_ret; eauto with encode.
 Qed.
 
 Lemma pure_eval_lor η e1 e2 (φ1 φ2 φ : Z → Prop) :
-  pure_enc (eval η e1) φ1 →
-  pure_enc (eval η e2) φ2 →
+  pure (eval η e1) ##φ1 ⊥ →
+  pure (eval η e2) ##φ2 ⊥ →
   (∀ z1 z2, φ1 z1 → φ2 z2 → φ (Z.lor z1 z2)) →
-  pure_enc (eval η (EIntLor e1 e2)) φ.
+  pure (eval η (EIntLor e1 e2)) ##φ ⊥.
 Proof.
   intros. simpl_eval. eapply pure_enc_par_as_int; eauto. intros.
   eapply pure_enc_ret; eauto with encode.
 Qed.
 
 Lemma pure_eval_lxor η e1 e2 (φ1 φ2 φ : Z → Prop) :
-  pure_enc (eval η e1) φ1 →
-  pure_enc (eval η e2) φ2 →
+  pure (eval η e1) ##φ1 ⊥ →
+  pure (eval η e2) ##φ2 ⊥ →
   (∀ z1 z2, φ1 z1 → φ2 z2 → φ (Z.lxor z1 z2)) →
-  pure_enc (eval η (EIntLxor e1 e2)) φ.
+  pure (eval η (EIntLxor e1 e2)) ##φ ⊥.
 Proof.
   intros. simpl_eval. eapply pure_enc_par_as_int; eauto. intros.
   eapply pure_enc_ret; eauto with encode.
 Qed.
 
 Lemma pure_eval_lsl η e1 e2 (φ1 φ2 φ : Z → Prop) :
-  pure_enc (eval η e1) φ1 →
-  pure_enc (eval η e2) φ2 →
+  pure (eval η e1) ##φ1 ⊥ →
+  pure (eval η e2) ##φ2 ⊥ →
   (∀ z1, φ1 z1 → representable z1) →
   (∀ z2, φ2 z2 → in_shift_range z2) →
   (∀ z1 z2, φ1 z1 → φ2 z2 → φ (Z.shiftl z1 z2)) →
-  pure_enc (eval η (EIntLsl e1 e2)) φ.
+  pure (eval η (EIntLsl e1 e2)) ##φ ⊥.
 Proof.
   intros. simpl_eval. eapply pure_enc_par_as_int; eauto. intros.
   apply pure_if_in_shift_range; auto.
@@ -331,12 +332,12 @@ Proof.
 Qed.
 
 Lemma pure_eval_lsr η e1 e2 (φ1 φ2 φ : Z → Prop) :
-  pure_enc (eval η e1) φ1 →
-  pure_enc (eval η e2) φ2 →
+  pure (eval η e1) ##φ1 ⊥ →
+  pure (eval η e2) ##φ2 ⊥ →
   (∀ z1, φ1 z1 → urepresentable z1) →
   (∀ z2, φ2 z2 → in_shift_range z2) →
   (∀ z1 z2, φ1 z1 → φ2 z2 → φ (Z.shiftr z1 z2)) →
-  pure_enc (eval η (EIntLsr e1 e2)) φ.
+  pure (eval η (EIntLsr e1 e2)) ##φ ⊥.
 Proof.
   intros. simpl_eval. eapply pure_enc_par_as_int; eauto. intros.
   apply pure_if_in_shift_range; auto.
@@ -344,12 +345,12 @@ Proof.
 Qed.
 
 Lemma pure_eval_asr η e1 e2 (φ1 φ2 φ : Z → Prop) :
-  pure_enc (eval η e1) φ1 →
-  pure_enc (eval η e2) φ2 →
+  pure (eval η e1) ##φ1 ⊥ →
+  pure (eval η e2) ##φ2 ⊥ →
   (∀ z1, φ1 z1 → representable z1) →
   (∀ z2, φ2 z2 → in_shift_range z2) →
   (∀ z1 z2, φ1 z1 → φ2 z2 → φ (Z.shiftr z1 z2)) →
-  pure_enc (eval η (EIntAsr e1 e2)) φ.
+  pure (eval η (EIntAsr e1 e2)) ##φ ⊥.
 Proof.
   intros. simpl_eval. eapply pure_enc_par_as_int; eauto. intros.
   apply pure_if_in_shift_range; auto.
@@ -358,10 +359,19 @@ Qed.
 
 (* Helper lemmas for operations on Booleans. *)
 
+Lemma pure_as_bool (m : microvx) (φ : bool → Prop) ψ :
+  pure m ##φ ψ →
+  pure (as_bool m) φ ψ.
+Proof.
+  intro H.
+  eapply pure_bind_conseq; eauto.
+  intros [] ([] & E & Hb); discriminate || rewrite E; with_strategy transparent [val_as_bool] by constructor.
+Qed.
+
 Lemma pure_enc_bind_as_bool {A} m (φ : bool → Prop) (ψ : A → Prop) (k : bool → micro A exn) :
-  pure_enc m φ →
-  (∀ b : bool, φ b → pure (k b) ψ (λ _, False)) →
-  pure (bind (as_bool m) k) ψ (λ _, False).
+  pure m ##φ ⊥ →
+  (∀ b : bool, φ b → pure (k b) ψ ⊥) →
+  pure (bind (as_bool m) k) ψ ⊥.
 Proof.
   intros Hm Hp. apply pure_bind, pure_as_bool.
   apply (pure_mono_ret _ Hm). intros ? (b & -> & Hb).
@@ -371,18 +381,18 @@ Qed.
 (* Primitive operations on Booleans. *)
 
 Lemma pure_eval_negb η e (φ ψ : bool → Prop) :
-  pure_enc (eval η e) φ →
+  pure (eval η e) ##φ ⊥ →
   (∀ b, φ b → ψ (negb b)) →
-  pure_enc (eval η (EBoolNeg e)) ψ.
+  pure (eval η (EBoolNeg e)) ##ψ ⊥.
 Proof.
   intros He Hp. simpl_eval.
   eapply pure_enc_bind_as_bool; eauto. intros b Hb. apply pure_ret. eauto with encode.
 Qed.
 
 Lemma pure_eval_not η e (φ ψ : Prop → Prop) :
-  pure_enc (eval η e) φ →
+  pure (eval η e) ##φ ⊥ →
   (∀ P, φ P → ψ (¬P)) →
-  pure_enc (eval η (EBoolNeg e)) ψ.
+  pure (eval η (EBoolNeg e)) ##ψ ⊥.
 Proof.
   intros He Hp. simpl_eval.
   eapply pure_bind.
@@ -400,13 +410,13 @@ Qed.
 
 Lemma pure_eval_let_pair `{Encode A1, Encode A2} `{Encode X}
   p1 p2 e1 e2 η (ψ : X -> Prop) :
-  pure_enc (eval η e1) (λ '((v1, v2) : A1 * A2),
-      pure_enc (
+  pure (eval η e1) ##(λ '((v1, v2) : A1 * A2),
+      pure (
           δ ← widen (irrefutably_extend [] p1 #v1);
           θ ← widen (irrefutably_extend δ p2 #v2);
           eval (θ ++ η) e2
-        ) ψ) ->
-  pure_enc (eval η (ELet1 (PPair p1 p2) e1 e2)) ψ.
+        ) ##ψ ⊥) ⊥ ->
+  pure (eval η (ELet1 (PPair p1 p2) e1 e2)) ##ψ ⊥.
 Proof.
   (* This proof is a long rewriting sequence, which makes some sense as it is
   not the standard method to prove a let binding, but rather a way to reduce the
@@ -441,9 +451,9 @@ Qed.
 
 Lemma pure_eval_let `{Encode A1, Encode B} η x e1 e
   (φ1 : A1 → Prop) (ψ : B → Prop) :
-  pure_enc (eval η e1) φ1 →
-  (∀ a1, φ1 a1 → pure_enc (eval ((x, #a1) :: η) e) ψ) →
-  pure_enc (eval η (ELet1Var x e1 e)) ψ.
+  pure (eval η e1) ##φ1 ⊥ →
+  (∀ a1, φ1 a1 → pure (eval ((x, #a1) :: η) e) ##ψ ⊥) →
+  pure (eval η (ELet1Var x e1 e)) ##ψ ⊥.
 Proof.
   intros He1 He.
   simpl_eval.
@@ -460,9 +470,9 @@ Qed.
 
 Lemma pure_eval_let' `{Encode A1, Encode B} η x e1 e
   (a1 : A1) (ψ : B → Prop) :
-  pure_enc (eval η e1) (λ x, x = a1) →
-  pure_enc (eval ((x, #a1) :: η) e) ψ →
-  pure_enc (eval η (ELet1Var x e1 e)) ψ.
+  pure (eval η e1) ##(λ x, x = a1) ⊥ →
+  pure (eval ((x, #a1) :: η) e) ##ψ ⊥ →
+  pure (eval η (ELet1Var x e1 e)) ##ψ ⊥.
 Proof.
   intros He1 He2.
   eapply pure_eval_let; eauto.
@@ -471,20 +481,34 @@ Qed.
 
 (* Conditionals. *)
 
+(* TODO fix inconsistent naming *)
+Lemma pure_ifthenelse_bool η e e1 e2 φ φb ψ :
+  pure (eval η e) ##φb ψ →
+  (φb true  → pure (eval η e1) φ ψ) →
+  (φb false → pure (eval η e2) φ ψ) →
+  pure (eval η (EIfThenElse e e1 e2)) φ ψ.
+Proof.
+  simpl.
+  intros Hb Ht Hf.
+  simpl_eval.
+  eapply pure_bind_conseq. apply pure_as_bool. apply Hb.
+  intros []; auto.
+Qed.
+
 Lemma pure_eval_ifthenelse_bool `{Encode A} η e e1 e2 (φ : bool → Prop) (ψ : A → Prop) :
-  pure_enc (eval η e) φ →
-  (φ true  → pure_enc (eval η e1) ψ) →
-  (φ false → pure_enc (eval η e2) ψ) →
-  pure_enc (eval η (EIfThenElse e e1 e2)) ψ.
+  pure (eval η e) ##φ ⊥ →
+  (φ true  → pure (eval η e1) ##ψ ⊥) →
+  (φ false → pure (eval η e2) ##ψ ⊥) →
+  pure (eval η (EIfThenElse e e1 e2)) ##ψ ⊥.
 Proof.
   intros. eapply pure_ifthenelse_bool; eauto.
 Qed.
 
 Lemma pure_eval_ifthenelse `{Encode A} η e e1 e2 (P : Prop) (ψ : A → Prop) :
-  pure_enc (eval η e) (λ P', P' <-> P) →
-  (P → pure_enc (eval η e1) ψ) →
-  (~ P → pure_enc (eval η e2) ψ) →
-  pure_enc (eval η (EIfThenElse e e1 e2)) ψ.
+  pure (eval η e) ##(λ P', P' <-> P) ⊥ →
+  (P → pure (eval η e1) ##ψ ⊥) →
+  (~ P → pure (eval η e2) ##ψ ⊥) →
+  pure (eval η (EIfThenElse e e1 e2)) ##ψ ⊥.
 Proof.
   intros He He1 He2.
   eapply pure_ifthenelse.
@@ -498,12 +522,12 @@ Qed.
 (* Helper lemma for Boolean operations *)
 
 Lemma pure_eval_comparison_operator `{Encode A} η e1 e2 (x1 x2 : Z) (f : val → val → micro bool exn) b a (φ : A → Prop) :
-  pure_enc (eval η e1) (λ x1' : Z, x1' = x1) →
-  pure_enc (eval η e2) (λ x2' : Z, x2' = x2) →
+  pure (eval η e1) ##(λ x1' : Z, x1' = x1) ⊥ →
+  pure (eval η e2) ##(λ x2' : Z, x2' = x2) ⊥ →
   f #x1 #x2 = ret b →
   #a = #b →
   φ a →
-  pure_enc (Par (eval η e1) (eval η e2) (pfbind inject2 (λ '(v1, v2), 'b ← f v1 v2; ret (VBool b)))) φ.
+  pure (Par (eval η e1) (eval η e2) (pfbind inject2 (λ '(v1, v2), 'b ← f v1 v2; ret (VBool b)))) ##φ ⊥.
 Proof.
   intros He1 He2 Ef Ea Ha.
   eapply pure_Par_conseq_ret; eauto.
@@ -517,12 +541,12 @@ Qed.
 (* Boolean operations *)
 
 Lemma pure_eval_EOpLe η e1 e2 (x1 x2 : Z) :
-  pure_enc (eval η e1) (λ x1', x1' = x1) ->
-  pure_enc (eval η e2) (λ x2', x2' = x2) ->
+  pure (eval η e1) ##(λ x1', x1' = x1) ⊥ ->
+  pure (eval η e2) ##(λ x2', x2' = x2) ⊥ ->
   (* Representability hypotheses last for [x1] and [x2] evar initialisation *)
   representable x1 ->
   representable x2 ->
-  pure_enc (eval η (EOpLe e1 e2)) (λ P, P <-> (x1 <= x2)%Z).
+  pure (eval η (EOpLe e1 e2)) ##(λ P, P <-> (x1 <= x2)%Z) ⊥.
 Proof.
   intros He1 He2 Hx1 Hx2. simpl_eval.
   eapply pure_eval_comparison_operator; eauto.
@@ -531,23 +555,23 @@ Proof.
 Qed.
 
 Lemma pure_eval_EOpLe_bool η e1 e2 (x1 x2 : Z) :
-  pure_enc (eval η e1) (λ x1', x1' = x1) ->
-  pure_enc (eval η e2) (λ x2', x2' = x2) ->
+  pure (eval η e1) ##(λ x1', x1' = x1) ⊥ ->
+  pure (eval η e2) ##(λ x2', x2' = x2) ⊥ ->
   representable x1 ->
   representable x2 ->
-  pure_enc (eval η (EOpLe e1 e2)) (λ (b : bool), b <-> (x1 <= x2)).
+  pure (eval η (EOpLe e1 e2)) ##(λ (b : bool), b <-> (x1 <= x2)) ⊥.
 Proof.
   intros. eapply pure_mono_ret. eapply pure_eval_EOpLe; eauto.
   intros _ (P & -> & HP). exists (truth P). by rewrite <-HP, encode_truth, Is_true_truth.
 Qed.
 
 Lemma pure_eval_EOpLt η e1 e2 (x1 x2 : Z) :
-  pure_enc (eval η e1) (λ x1', x1' = x1) ->
-  pure_enc (eval η e2) (λ x2', x2' = x2) ->
+  pure (eval η e1) ##(λ x1', x1' = x1) ⊥ ->
+  pure (eval η e2) ##(λ x2', x2' = x2) ⊥ ->
   (* Representability hypotheses last for [x1] and [x2] evar initialisation *)
   representable x1 ->
   representable x2 ->
-  pure_enc (eval η (EOpLt e1 e2)) (λ P, P <-> (x1 < x2)%Z).
+  pure (eval η (EOpLt e1 e2)) ##(λ P, P <-> (x1 < x2)%Z) ⊥.
 Proof.
   intros He1 He2 Hx1 Hx2. simpl_eval.
   eapply pure_eval_comparison_operator; eauto.
@@ -556,24 +580,24 @@ Proof.
 Qed.
 
 Lemma pure_eval_EOpLt_bool η e1 e2 (x1 x2 : Z) :
-  pure_enc (eval η e1) (λ x1', x1' = x1) ->
-  pure_enc (eval η e2) (λ x2', x2' = x2) ->
+  pure (eval η e1) ##(λ x1', x1' = x1) ⊥ ->
+  pure (eval η e2) ##(λ x2', x2' = x2) ⊥ ->
   (* Representability hypotheses last for [x1] and [x2] evar initialisation *)
   representable x1 ->
   representable x2 ->
-  pure_enc (eval η (EOpLt e1 e2)) (λ (b : bool), b <-> (x1 < x2)).
+  pure (eval η (EOpLt e1 e2)) ##(λ (b : bool), b <-> (x1 < x2)) ⊥.
 Proof.
   intros. eapply pure_mono_ret. eapply pure_eval_EOpLt; eauto.
   intros _ (P & -> & HP). exists (truth P). by rewrite <-HP, encode_truth, Is_true_truth.
 Qed.
 
 Lemma pure_eval_EOpGt η e1 e2 (x1 x2 : Z) :
-  pure_enc (eval η e1) (λ x1', x1' = x1) ->
-  pure_enc (eval η e2) (λ x2', x2' = x2) ->
+  pure (eval η e1) ##(λ x1', x1' = x1) ⊥ ->
+  pure (eval η e2) ##(λ x2', x2' = x2) ⊥ ->
   (* Representability hypotheses last for [x1] and [x2] evar initialisation *)
   representable x1 ->
   representable x2 ->
-  pure_enc (eval η (EOpGt e1 e2)) (λ P, P <-> (x1 > x2)%Z).
+  pure (eval η (EOpGt e1 e2)) ##(λ P, P <-> (x1 > x2)%Z) ⊥.
 Proof.
   intros He1 He2 Hx1 Hx2. simpl_eval.
   eapply pure_eval_comparison_operator; eauto.
@@ -582,24 +606,24 @@ Proof.
 Qed.
 
 Lemma pure_eval_EOpGt_bool η e1 e2 (x1 x2 : Z) :
-  pure_enc (eval η e1) (λ x1', x1' = x1) ->
-  pure_enc (eval η e2) (λ x2', x2' = x2) ->
+  pure (eval η e1) ##(λ x1', x1' = x1) ⊥ ->
+  pure (eval η e2) ##(λ x2', x2' = x2) ⊥ ->
   (* Representability hypotheses last for [x1] and [x2] evar initialisation *)
   representable x1 ->
   representable x2 ->
-  pure_enc (eval η (EOpGt e1 e2)) (λ (b : bool), b <-> (x1 > x2)).
+  pure (eval η (EOpGt e1 e2)) ##(λ (b : bool), b <-> (x1 > x2)) ⊥.
 Proof.
   intros. eapply pure_mono_ret. eapply pure_eval_EOpGt; eauto.
   intros _ (P & -> & HP). exists (truth P). by rewrite <-HP, encode_truth, Is_true_truth.
 Qed.
 
 Lemma pure_eval_EOpGe η e1 e2 (x1 x2 : Z) :
-  pure_enc (eval η e1) (λ x1', x1' = x1) ->
-  pure_enc (eval η e2) (λ x2', x2' = x2) ->
+  pure (eval η e1) ##(λ x1', x1' = x1) ⊥ ->
+  pure (eval η e2) ##(λ x2', x2' = x2) ⊥ ->
   (* Representability hypotheses last for [x1] and [x2] evar initialisation *)
   representable x1 ->
   representable x2 ->
-  pure_enc (eval η (EOpGe e1 e2)) (λ P, P <-> (x1 >= x2)%Z).
+  pure (eval η (EOpGe e1 e2)) ##(λ P, P <-> (x1 >= x2)%Z) ⊥.
 Proof.
   intros He1 He2 Hx1 Hx2. simpl_eval.
   eapply pure_eval_comparison_operator; eauto.
@@ -608,24 +632,24 @@ Proof.
 Qed.
 
 Lemma pure_eval_EOpGe_bool η e1 e2 (x1 x2 : Z) :
-  pure_enc (eval η e1) (λ x1', x1' = x1) ->
-  pure_enc (eval η e2) (λ x2', x2' = x2) ->
+  pure (eval η e1) ##(λ x1', x1' = x1) ⊥ ->
+  pure (eval η e2) ##(λ x2', x2' = x2) ⊥ ->
   (* Representability hypotheses last for [x1] and [x2] evar initialisation *)
   representable x1 ->
   representable x2 ->
-  pure_enc (eval η (EOpGe e1 e2)) (λ (b : bool), b <-> (x1 >= x2)).
+  pure (eval η (EOpGe e1 e2)) ##(λ (b : bool), b <-> (x1 >= x2)) ⊥.
 Proof.
   intros. eapply pure_mono_ret. eapply pure_eval_EOpGe; eauto.
   intros _ (P & -> & HP). exists (truth P). by rewrite <-HP, encode_truth, Is_true_truth.
 Qed.
 
 Lemma pure_eval_EOpEq η e1 e2 (x1 x2 : Z) :
-  pure_enc (eval η e1) (λ x1', x1' = x1) ->
-  pure_enc (eval η e2) (λ x2', x2' = x2) ->
+  pure (eval η e1) ##(λ x1', x1' = x1) ⊥ ->
+  pure (eval η e2) ##(λ x2', x2' = x2) ⊥ ->
   (* Representability hypotheses last for [x1] and [x2] evar initialisation *)
   representable x1 ->
   representable x2 ->
-  pure_enc (eval η (EOpEq e1 e2)) (λ P, P <-> (x1 = x2)%Z).
+  pure (eval η (EOpEq e1 e2)) ##(λ P, P <-> (x1 = x2)%Z) ⊥.
 Proof.
   intros He1 He2 Hx1 Hx2. simpl_eval.
   eapply pure_eval_comparison_operator; eauto.
@@ -634,24 +658,24 @@ Proof.
 Qed.
 
 Lemma pure_eval_EOpEq_bool η e1 e2 (x1 x2 : Z) :
-  pure_enc (eval η e1) (λ x1', x1' = x1) ->
-  pure_enc (eval η e2) (λ x2', x2' = x2) ->
+  pure (eval η e1) ##(λ x1', x1' = x1) ⊥ ->
+  pure (eval η e2) ##(λ x2', x2' = x2) ⊥ ->
   (* Representability hypotheses last for [x1] and [x2] evar initialisation *)
   representable x1 ->
   representable x2 ->
-  pure_enc (eval η (EOpEq e1 e2)) (λ (b : bool), b <-> (x1 = x2)).
+  pure (eval η (EOpEq e1 e2)) ##(λ (b : bool), b <-> (x1 = x2)) ⊥.
 Proof.
   intros. eapply pure_mono_ret. eapply pure_eval_EOpEq; eauto.
   intros _ (P & -> & HP). exists (truth P). by rewrite <-HP, encode_truth, Is_true_truth.
 Qed.
 
 Lemma pure_eval_EOpNe η e1 e2 (x1 x2 : Z) :
-  pure_enc (eval η e1) (λ x1', x1' = x1) ->
-  pure_enc (eval η e2) (λ x2', x2' = x2) ->
+  pure (eval η e1) ##(λ x1', x1' = x1) ⊥ ->
+  pure (eval η e2) ##(λ x2', x2' = x2) ⊥ ->
   (* Representability hypotheses last for [x1] and [x2] evar initialisation *)
   representable x1 ->
   representable x2 ->
-  pure_enc (eval η (EOpNe e1 e2)) (λ P, P <-> (x1 <> x2)%Z).
+  pure (eval η (EOpNe e1 e2)) ##(λ P, P <-> (x1 <> x2)%Z) ⊥.
 Proof.
   intros He1 He2 Hx1 Hx2. simpl_eval.
   eapply pure_eval_comparison_operator; eauto.
@@ -660,12 +684,12 @@ Proof.
 Qed.
 
 Lemma pure_eval_EOpNe_bool η e1 e2 (x1 x2 : Z) :
-  pure_enc (eval η e1) (λ x1', x1' = x1) ->
-  pure_enc (eval η e2) (λ x2', x2' = x2) ->
+  pure (eval η e1) ##(λ x1', x1' = x1) ⊥ ->
+  pure (eval η e2) ##(λ x2', x2' = x2) ⊥ ->
   (* Representability hypotheses last for [x1] and [x2] evar initialisation *)
   representable x1 ->
   representable x2 ->
-  pure_enc (eval η (EOpNe e1 e2)) (λ (b : bool), b <-> (x1 <> x2)).
+  pure (eval η (EOpNe e1 e2)) ##(λ (b : bool), b <-> (x1 <> x2)) ⊥.
 Proof.
   intros. eapply pure_mono_ret. eapply pure_eval_EOpNe; eauto.
   intros _ (P & -> & HP). exists (truth P). by rewrite <-HP, encode_truth, Is_true_truth.
@@ -674,8 +698,8 @@ Qed.
 (* Runtime assertions. *)
 
 Lemma pure_eval_assert_bool η e :
-  pure_enc (eval η e) (λ b, b = true) →
-  pure_enc (eval η (EAssert e)) (λ (_ : unit), True).
+  pure (eval η e) ##(λ b, b = true) ⊥ →
+  pure (eval η (EAssert e)) ##(λ (_ : unit), True) ⊥.
 Proof.
   intros He.
   eapply pure_mono_ret.
@@ -683,12 +707,12 @@ Proof.
   eapply pure_mono_ret.
   eapply He.
   - by intros _ (V & -> & ->).
-  - intros _ ->. eauto.
+  - intros _ ->. eauto with encode.
 Qed.
 
 Lemma pure_eval_assert_Prop η e :
-  pure_enc (eval η e) (λ P : Prop, P) →
-  pure_enc (eval η (EAssert e)) (λ (_ : unit), True).
+  pure (eval η e) ##(λ P : Prop, P) ⊥ →
+  pure (eval η (EAssert e)) ##(λ (_ : unit), True) ⊥.
 Proof.
   intros He.
   eapply pure_mono_ret.
@@ -697,15 +721,15 @@ Proof.
   eapply He.
   - intros _ (P & -> & HP).
     unfold encode, Encode_bool, Encode_Prop. by rewrite truth_true.
-  - intros _ ->. eauto.
+  - intros _ ->. eauto with encode.
 Qed.
 
 (* Sequencing of pure computations. *)
 
 Lemma pure_eval_seq' `{Encode A} η e1 e2 (ψ : A -> Prop) :
-  pure (eval η e1) (λ _, True) (λ _, False) ->
-  pure_enc (eval η e2) ψ ->
-  pure_enc (eval η (ESeq e1 e2)) ψ.
+  pure (eval η e1) (λ _, True) ⊥ ->
+  pure (eval η e2) ##ψ ⊥ ->
+  pure (eval η (ESeq e1 e2)) ##ψ ⊥.
 Proof.
   intros He1 He2.
   apply pure_seq.
@@ -714,9 +738,9 @@ Proof.
 Qed.
 
 Lemma pure_eval_seq `{Encode A} `{Encode B} η e1 e2 (ψ : A -> Prop) :
-  pure_enc (eval η e1) (λ _ : B, True) ->
-  pure_enc (eval η e2) ψ ->
-  pure_enc (eval η (ESeq e1 e2)) ψ.
+  pure (eval η e1) ##(λ _ : B, True) ⊥ ->
+  pure (eval η e2) ##ψ ⊥ ->
+  pure (eval η (ESeq e1 e2)) ##ψ ⊥.
 Proof.
   intros He1 He2.
   apply pure_seq.
@@ -727,16 +751,16 @@ Qed.
 Lemma pure_eval_mexpr_struct (η δ whatenv : env) items (ψ : val -> Prop) :
   simp (eval_sitems (η, []) items) (ret (whatenv, δ)) ->
   ψ (VStruct δ) ->
-  pure_enc (eval_mexpr η (MStruct items)) ψ.
+  pure (eval_mexpr η (MStruct items)) ##ψ ⊥.
 Proof.
   intros. simpl_eval_mexpr.
-  eapply pure_simp; [ simp | eauto using pure_ret ].
+  eapply pure_simp; [ simp | eauto using pure_ret with encode ].
 Qed.
 
 Lemma pure_eval_mexpr_coerc η me c v (ψ : val -> Prop):
   simp (eval_mexpr η me) (ret v) ->
-  pure_enc (coerce c v) ψ ->
-  pure_enc (eval_mexpr η (MCoercion me c)) ψ.
+  pure (coerce c v) ##ψ ⊥ ->
+  pure (eval_mexpr η (MCoercion me c)) ##ψ ⊥.
 Proof.
   intros Hme Hc. simpl_eval_mexpr. eapply pure_bind.
   eapply pure_simp; eauto.
@@ -747,17 +771,17 @@ Proof.
 Qed.
 
 Lemma pure_eval_path `{Encode A} η π (ψ : A -> Prop) :
-  pure_enc (lookup_path η π) ψ ->
-  pure_enc (eval η (EPath π)) ψ.
+  pure (lookup_path η π) ##ψ ⊥ ->
+  pure (eval η (EPath π)) ##ψ ⊥.
 Proof.
   simpl_eval.
   apply pure_widen.
 Qed.
 
 Lemma pure_eval_ret_concat `{Encode A} e δ η (ψ : A -> Prop) :
-  pure_enc (eval (δ ++ η) e) ψ ->
-  pure_enc (θ ← ret (δ ++ η);
-        eval θ e) ψ.
+  pure (eval (δ ++ η) e) ##ψ ⊥ ->
+  pure (θ ← ret (δ ++ η);
+        eval θ e) ##ψ ⊥.
 Proof.
   tauto.
 Qed.
@@ -765,17 +789,17 @@ Qed.
 Lemma pure_eval_const `{Encode X} η c x (ψ : X -> Prop) :
   VConstant c = #x ->
   ψ x ->
-  pure_enc (eval η (EConstant c)) ψ.
+  pure (eval η (EConstant c)) ##ψ ⊥.
 Proof.
   intros.
   eapply pure_simp. simp.
-  eauto using pure_ret.
+  eauto using pure_ret with encode.
 Qed.
 
 Lemma pure_eval_data `{Encode Y} η c e y (ψ : Y -> Prop) :
-  pure_enc (eval η e) (λ v', VData c v' = #y) ->
+  pure (eval η e) ##(λ v', VData c v' = #y) ⊥ ->
   ψ y ->
-  pure_enc (eval η (EData c e)) ψ.
+  pure (eval η (EData c e)) ##ψ ⊥.
 Proof.
   intros He Hy.
   simpl_eval.
@@ -789,10 +813,10 @@ Class CRel1 {A : Type} (X : Type) `{Encode A, Encode X}
   (c : string) (C : A -> X) := { }.
 
 Lemma pure_eval_data1 `{CRel1 A1 X c C} (η : env) (e : expr) (ψ : X → Prop) :
-  pure_enc (eval η e)
-    (λ x,
-      VData c (VTuple1 #x) = #(C x) /\ ψ (C x)) ->
-  pure_enc (eval η (EData c (ETuple [e]))) ψ.
+  pure (eval η e)
+    ##(λ x,
+      VData c (VTuple1 #x) = #(C x) /\ ψ (C x)) ⊥ ->
+  pure (eval η (EData c (ETuple [e]))) ##ψ ⊥.
 Proof.
   intros He.
   simpl_eval.
@@ -800,7 +824,7 @@ Proof.
   eapply (pure_mono_ret _ He).
   intros _ (? & -> & ? & ?).
   repeat apply pure_ret || apply pure_bind.
-  eauto.
+  eauto with encode.
 Qed.
 
 Class CRel2 (A1 A2 X : Type) `{Encode A1, Encode A2, Encode X}
@@ -811,17 +835,17 @@ Class CRel2 (A1 A2 X : Type) `{Encode A1, Encode A2, Encode X}
    does not to remove the vector notation from Coq's parser. *)
 
 Lemma pure_eval_data2 `{CRel2 A1 A2 X c C} (η : env) (e : expr) (ψ : X → Prop) :
-  pure_enc (eval η e)
-    (λ '(x, y),
-      VData c (VTuple [encode x; #y]) = #(C x y) /\ ψ (C x y)) ->
-  pure_enc (eval η (EData c e)) ψ.
+  pure (eval η e)
+    ##(λ '(x, y),
+      VData c (VTuple [encode x; #y]) = #(C x y) /\ ψ (C x y)) ⊥ ->
+  pure (eval η (EData c e)) ##ψ ⊥.
 Proof.
   intros He.
   simpl_eval. apply pure_bind.
   eapply (pure_mono_ret _ He).
   intros _ ((?, ?) & -> & ? & ?).
   repeat apply pure_ret || apply pure_bind.
-  eauto.
+  eauto with encode.
 Qed.
 
 (* Example usage of the CRel typeclasses:
@@ -833,32 +857,32 @@ Class CRel3 {A1 A2 A3 : Type} (X : Type) `{Encode A1, Encode A2, Encode A3, Enco
   (c : string) (C : A1 -> A2 -> A3 -> X) := { }.
 
 Lemma pure_eval_data3 `{CRel3 A1 A2 A3 X c C} (η : env) (e : expr) (ψ : X → Prop) :
-  pure_enc (eval η e)
-    (λ '(x, y, z),
-      VData c (VTuple ([encode x; #y; #z])) = #(C x y z) /\ ψ (C x y z)) ->
-  pure_enc (eval η (EData c e)) ψ.
+  pure (eval η e)
+    ##(λ '(x, y, z),
+      VData c (VTuple ([encode x; #y; #z])) = #(C x y z) /\ ψ (C x y z)) ⊥ ->
+  pure (eval η (EData c e)) ##ψ ⊥.
 Proof.
   intros He.
   simpl_eval. apply pure_bind.
   eapply (pure_mono_ret _ He).
   intros ? (((?, ?), ?) & -> & ? & ?).
   repeat apply pure_ret || apply pure_bind.
-  eauto.
+  eauto with encode.
 Qed.
 
 Class CRel4 (A1 A2 A3 A4 X : Type) `{Encode A1, Encode A2, Encode A3, Encode A4, Encode X}
   (c : string) (C : A1 -> A2 -> A3 -> A4 -> X) := { }.
 
 Lemma pure_eval_data4 `{CRel4 A1 A2 A3 A4 X c C} (η : env) (e : expr) (ψ : X → Prop) :
-  pure_enc (eval η e)
-    (λ '(x, y, z, w),
-      VData c (VTuple ([encode x; #y; #z; #w])) = #(C x y z w) /\ ψ (C x y z w)) ->
-  pure_enc (eval η (EData c e)) ψ.
+  pure (eval η e)
+    ##(λ '(x, y, z, w),
+      VData c (VTuple ([encode x; #y; #z; #w])) = #(C x y z w) /\ ψ (C x y z w)) ⊥ ->
+  pure (eval η (EData c e)) ##ψ ⊥.
 Proof.
   intros He.
   simpl_eval. apply pure_bind.
   eapply (pure_mono_ret _ He).
   intros ? ((((?, ?), ?), ?) & -> & ? & ?).
   repeat apply pure_ret || apply pure_bind.
-  eauto.
+  eauto with encode.
 Qed.
